chore: unify `induction` tactic

tests/lean/run/induction1.lean
@@ -1,5 +1,5 @@
 @[recursor 4]
-def Or.elim2 {p q r : Prop} (major : p ∨ q) (left : p → r) (right : q → r) : r :=
+def Or.elim2 {p q : Prop} {r : p ∨ q → Prop} (major : p ∨ q) (left : (h : p) → r (Or.inl h)) (right : (h : q) → r (Or.inr h)) : r major :=
   match  major with
   | Or.inl h => left h
   | Or.inr h => right h
@@ -26,29 +26,29 @@ induction h with
 | inl h1 => exact Or.inr h1
 
 theorem tst2 {p q : Prop } (h : p ∨ q) : q ∨ p := by
-induction h using elim2 with
+induction h using Or.elim2 with
 | left _  => apply Or.inr; assumption
 | right _ => apply Or.inl; assumption
 
 theorem tst2b {p q : Prop } (h : p ∨ q) : q ∨ p := by
-induction h using elim2 with
+induction h using Or.elim2 with
 | left => apply Or.inr; assumption
 | _ => apply Or.inl; assumption
 
 theorem tst3 {p q : Prop } (h : p ∨ q) : q ∨ p := by
-induction h using elim2 with
+induction h using Or.elim2 with
 | right h => exact Or.inl h
 | left h  => exact Or.inr h
 
 theorem tst4 {p q : Prop } (h : p ∨ q) : q ∨ p := by
-induction h using elim2 with
+induction h using Or.elim2 with
 | right h => ?myright
 | left h  => ?myleft
 case myleft  => exact Or.inr h
 case myright => exact Or.inl h
 
 theorem tst5 {p q : Prop } (h : p ∨ q) : q ∨ p := by
-induction h using elim2 with
+induction h using Or.elim2 with
 | right h => _
 | left h  =>
   refine Or.inr ?_
@@ -64,13 +64,13 @@ by {
 
 theorem tst7 {α : Type} (xs : List α) (h : (a : α) → (as : List α) → xs ≠ a :: as) : xs = [] :=
 by {
-  induction xs with
+  induction xs generalizing h with
   | nil          => exact rfl
   | cons z zs ih => exact absurd rfl (h z zs)
 }
 
 theorem tst8 {α : Type} (xs : List α) (h : (a : α) → (as : List α) → xs ≠ a :: as) : xs = [] := by {
-  induction xs;
+  induction xs generalizing h;
   exact rfl;
   exact absurd rfl $ h _ _
 }
@@ -111,7 +111,7 @@ theorem tst13 (x : Tree) (h : x = Tree.leaf₁) : x.isLeaf₁ = true := by
   | _     => injection h
 
 theorem tst14 (x : Tree) (h : x = Tree.leaf₁) : x.isLeaf₁ = true := by
-  induction x with
+  induction x generalizing h with
   | leaf₁ => rfl
   | _     => injection h
 
